proof/invariant-abstract/IpcCancel_AI.thy
@@ -2402,7 +2402,7 @@ lemma refill_unblock_check_obj_at_impossible':
    \<lbrace>\<lambda>s. P (obj_at P' p s)\<rbrace>"
   unfolding refill_unblock_check_def
   by (wpsimp wp: whileLoop_valid_inv update_sched_context_wp get_refills_wp
-           simp: refill_head_overlapping_loop_def merge_refills_def update_refill_hd_def
+           simp: refill_head_overlapping_loop_def merge_overlapping_refills_def update_refill_hd_def
                  refill_pop_head_def is_round_robin_def
     | clarsimp elim!: rsubst[where P=P] simp: obj_at_def)+
 
